src/Pyrosome/Compilers/SemanticsPreservingDef.v
@@ -1,0 +1,108 @@
+Set Implicit Arguments.
+
+Require Import Datatypes.String Lists.List.
+Import ListNotations.
+Open Scope string.
+Open Scope list.
+From Utils Require Import Utils.
+From Pyrosome.Theory Require Import Core.
+Import Core.Notations.
+
+Section WithVar.
+  Context (V : Type)
+          {V_Eqb : Eqb V}
+          {V_default : WithDefault V}.
+
+  Notation named_list := (@named_list V).
+  Notation named_map := (@named_map V).
+  Notation term := (@term V).
+  Notation ctx := (@ctx V).
+  Notation sort := (@sort V).
+  Notation subst := (@subst V).
+  Notation rule := (@rule V).
+  Notation lang := (@lang V).
+  
+  Notation eq_subst l :=
+    (eq_subst (Model:= core_model l)).
+  Notation eq_args l :=
+    (eq_args (Model:= core_model l)).
+  Notation wf_subst l :=
+    (wf_subst (Model:= core_model l)).
+  Notation wf_args l :=
+    (wf_args (Model:= core_model l)).
+  Notation wf_ctx l :=
+    (wf_ctx (Model:= core_model l)).
+
+  
+  Section WithModel.
+    Context {tgt_term tgt_sort : Type}
+      {tgt_Model : @Model V tgt_term tgt_sort}
+      (*TODO: should I make it so that these aren't necessary?*)
+      `{WithDefault tgt_term}
+      `{WithDefault tgt_sort}.
+
+    Existing Instance tgt_Model.
+
+    Section CompileJudgment.
+      Context (compile : term -> tgt_term)
+        (compile_sort : sort -> tgt_sort)
+        (compile_ctx : ctx -> named_list tgt_sort)
+        (compile_args : list term -> list tgt_term)
+        (compile_subst : subst -> named_list tgt_term)
+        (src : lang).
+      
+      (* First we specify the properties semantically,
+     then inductively on the compiler. TODO: prove equivalent
+       *)
+      Definition sort_wf_preserving_sem :=
+        forall c t,
+          wf_sort src c t ->
+          wf_ctx src c ->
+          Model.wf_sort (compile_ctx c) (compile_sort t).
+
+      Definition term_wf_preserving_sem :=
+        forall c e t,
+          wf_term src c e t ->
+          wf_ctx src c ->
+          Model.wf_term (compile_ctx c) (compile e) (compile_sort t).
+
+      Definition sort_eq_preserving_sem :=
+        forall c t1 t2,
+          eq_sort src c t1 t2 ->
+          wf_ctx src c ->
+          Model.eq_sort (compile_ctx c) (compile_sort t1) (compile_sort t2).
+      
+      Definition term_eq_preserving_sem :=
+        forall c t e1 e2,
+          eq_term src c t e1 e2 ->
+          wf_ctx src c ->
+          Model.eq_term (compile_ctx c) (compile_sort t) (compile e1) (compile e2).
+
+      Definition args_wf_preserving_sem :=
+        forall c s c',
+          wf_args src c s c' ->
+          wf_ctx src c ->
+          wf_ctx src c' ->
+          Model.wf_args (compile_ctx c) (compile_args s) (compile_ctx c').
+
+      Definition subst_eq_preserving_sem :=
+        forall c c' s1 s2,
+          eq_subst src c c' s1 s2 ->
+          wf_ctx src c ->
+          wf_ctx src c' ->
+          Model.eq_subst (compile_ctx c) (compile_ctx c') (compile_subst s1) (compile_subst s2).
+      
+      Definition ctx_wf_preserving_sem :=
+        forall c, wf_ctx src c -> Model.wf_ctx (compile_ctx c).
+
+      (*Set up to match the combined scheme for the judgment inductives *)
+      Definition semantics_preserving :=
+        sort_eq_preserving_sem /\ term_eq_preserving_sem /\ subst_eq_preserving_sem
+        /\ sort_wf_preserving_sem /\ term_wf_preserving_sem /\ args_wf_preserving_sem
+        /\ ctx_wf_preserving_sem.
+
+    End CompileJudgment.
+
+  End WithModel.
+
+End WithVar.
